polished teh semantics, time to start the proofs

hol/table_var_to_arithScript.sml
@@ -46,20 +46,12 @@ Type intvl_row = “:arith_lv option # (num # num) option # num # 'a action_expr
 (* None = Empty, Some (a,b) = Single [a,b] *)
 (* arith_lv from policy_arith_to_var*)
 
-
 Type intvl_table = “:('a intvl_row) list”;
 Type intvl_table_list = “:('a intvl_table ) list”;
 
-
-   
-
    
 val _ = Hol_datatype `
-   arith_atom_result = 
-    SingleAtom of arithm_atom
-  | UnionAtoms of arithm_atom => arithm_atom`;
-
-
+   arith_atom_result =  SingleAtom of arithm_atom | UnionAtoms of arithm_atom => arithm_atom`;
 
 val _ = Hol_datatype `
   pd_type = 
@@ -71,8 +63,6 @@ Type pd_type_struct = “: (string # pd_type) list”;
 
 
                                                                 
-
-
 Definition get_lval_def:
   get_lval (a_True) = NONE ∧
   get_lval (a_False) = NONE ∧
@@ -106,15 +96,10 @@ Definition resolve_pd_max_def:
       | _ => NONE
 End
 
-
         
-
 (* Convert atom_var to arithm_atom using m_e
    i.e. each cell in the line of var table will be converted
-   directly to an aritmetic atom via this def.
- *)
- 
-   (* edited this too much , REMOVE MAX FROM THIS DEF*)        
+   directly to an aritmetic atom via this def. *)       
 Definition atom_to_arith_def:
   (atom_to_arith m_e True = SOME (SingleAtom a_True)) ∧   
   (atom_to_arith m_e False = SOME (SingleAtom a_False)) ∧
@@ -139,7 +124,6 @@ Definition atom_to_arith_def:
 End
         
 
-
 Definition arith_to_interval_def:
   (arith_to_interval a_True max = Single 0 max) ∧
   (arith_to_interval a_False max = Empty) ∧
@@ -152,29 +136,6 @@ Definition arith_to_interval_def:
   (arith_to_interval (arithm_eq _ n) max = 
      if n < 0 ∨ n > max then Empty else Single n n)
 End
-        
-
-(*
-val test_true =  EVAL ``arith_to_interval a_True 100 = Single 0 100``;
-val test_false =  EVAL ``arith_to_interval a_False 100 = Empty``;
-
-val test_gt_normal =  EVAL ``arith_to_interval (arithm_gt (lv_x "x") 5) 10 = Single 6 10``;
-val test_gt_at_max =  EVAL ``arith_to_interval (arithm_gt (lv_x "x") 10) 10 = Empty``;
-val test_gt_above_max = EVAL ``arith_to_interval (arithm_gt (lv_x "x") 15) 10 = Empty``;
-val test_gt_at_zero = EVAL ``arith_to_interval (arithm_gt (lv_x "x") 0) 10 = Single 1 10``;
-
-val test_lt_normal = EVAL ``arith_to_interval (arithm_lt (lv_x "x") 5) 10 = Single 0 4``;
-val test_lt_at_zero = EVAL ``arith_to_interval (arithm_lt (lv_x "x") 0) 10 = Empty``;
-val test_lt_at_one = EVAL ``arith_to_interval (arithm_lt (lv_x "x") 1) 10 = Single 0 0``;
-val test_lt_above_max = EVAL ``arith_to_interval (arithm_lt (lv_x "x") 15) 10 = Single 0 10``;
-
-(* Equality tests *)
-val test_eq_normal = EVAL ``arith_to_interval (arithm_eq (lv_x "x") 5) 10 = Single 5 5``;
-val test_eq_at_max =  EVAL ``arith_to_interval (arithm_eq (lv_x "x") 10) 10 = Single 10 10``;
-val test_eq_below_zero = EVAL ``arith_to_interval (arithm_eq (lv_x "x") 0) 10 = Single 0 0``;
-val test_eq_above_max = EVAL ``arith_to_interval (arithm_eq (lv_x "x") 11) 10 = Empty``;
-*)
-
         
 
 Definition intersect_single_def:
@@ -235,85 +196,6 @@ Definition process_guard_def:
 End
 
 
-
-(*
-val test_mapping = “[("x", arithm_gt (lv_x "x") (5:num))]”;
-val test_max = “(10:num)”;
-
-val test_empty_input = EVAL ``process_guard ^test_mapping ^test_max True [] = []``;
-
-val test_failed_guard_conversion = EVAL ``process_guard ^test_mapping ^test_max (Var "y") [(NONE, SOME (2,8), 1, action "a")] = []``;
-
-val test_true_guard = EVAL ``process_guard ^test_mapping ^test_max True [(NONE, SOME (2,8), 1, action "a")] = [(NONE, SOME (2,8), 1, action "a")]``;
-
-val test_false_guard = EVAL ``process_guard ^test_mapping ^test_max False [(NONE, SOME (2,8), 1, action "a")] = [(NONE, NONE, 1, action "a")]``;
-        
-val test_single_atom_intersect = EVAL ``process_guard ^test_mapping ^test_max (Var "x") [(NONE, SOME (2,8), 1, action "a")]  = [(NONE, SOME (6,8), 1, action "a")]``;
-        
-val test_single_atom_no_intersect =  EVAL ``process_guard ^test_mapping ^test_max (Var "x") [(NONE, SOME (2,4), 1, action "a")]  = [(NONE, NONE, 1, action "a")]``;
-
-
-
-val test_mapping2 = “[("x", arithm_eq (lv_x "x") (5:num))]”;
-
-   
-val test_union_atom_guard =
-let
-    val guard = ``Not (Var "x"):atom_var``;
-    val input = ``[(NONE:arith_lv option, SOME (2:num,8:num), 1:num, 
-                    (action "a"):string action_expr)]``;      
-    val expected = ``[(NONE:arith_lv option, SOME (2:num,4:num), 1:num, 
-                      (action "a"):string action_expr);
-                     (NONE:arith_lv option, SOME (6:num,8:num), 1:num, 
-                      (action "a"):string action_expr)]``;
-  in
-    EVAL ``process_guard (^test_mapping2:(string # arithm_atom) list) 
-                         (^test_max:num) 
-                         ^guard 
-                         ^input = ^expected ``
-  end;
-
-
-val test_union_partial_intersect =
-  let
-    val guard = ``Not (Var "x"):atom_var``;
-    val input = ``[(NONE:arith_lv option, SOME (6:num,8:num), 1:num, 
-                   (action "a"):string action_expr)]``;
-    val expected = ``[(NONE:arith_lv option, SOME (6:num,8:num), 1:num, 
-                      (action "a"):string action_expr)]``;
-  in
-    EVAL ``process_guard ^test_mapping2 ^test_max ^guard ^input = ^expected ``
-  end;
-
-
-val test_mapping = “[("x", arithm_gt (lv_x "x") 5)] : (string # arithm_atom) list”
-    EVAL ``process_guard ^test_mapping ^test_max ^guard ^input ``
-
-
-  
-
-val test_no_current_interval =
-  EVAL ``process_guard ^test_mapping ^test_max True [(NONE, NONE, 1, action "a")]
-        = [(NONE, NONE, 1, action "a")]``;
-
-
-val test_multiple_rows =
-  EVAL ``process_guard ^test_mapping ^test_max (Var "x") 
-        [(NONE, SOME (2,8), 1, action "a"); (NONE, SOME (3,5), 2, action "b")]
-        = [(NONE, SOME (6,8), 1, action "a"); (NONE, NONE, 2, action "b")]``;
-
-
-val test_mapping3 = “[("x", arithm_eq (lv_x "x") (10:num))]”;
-
-  EVAL ``process_guard ^test_mapping3 ^test_max (Not(Var "x"))  [(NONE, SOME (0,10), 1, action "a")]``;
-
-        
-*)
-
-
-     
-
-
 (* processing guards recursively *)
 Definition process_guards_rec_def:
   (process_guards_rec m_e max  [] acc = acc) ∧
@@ -336,8 +218,6 @@ Definition get_lval_of_guard_in_me_def:
 End
 
 
-     
-
 Definition is_bool_or_unique_var_def:
   is_bool_or_unique_var m_e var_guards = 
     let lvals = FILTER IS_SOME (MAP (get_lval_of_guard_in_me m_e) var_guards) in
@@ -349,9 +229,7 @@ Definition is_bool_or_unique_var_def:
           else NONE              (* Different LVals detected *)
 End
 
-
-        
-        
+       
 Definition convert_line_def:
   (convert_line m_e pd_type ([], s, res) = SOME [(NONE, SOME (0,255), s, res)]) ∧  (* Default max *)
   (convert_line m_e pd_type (var_guards, s, res) =
@@ -360,18 +238,16 @@ Definition convert_line_def:
    | SOME (T, NONE) => (* all booleans, possibly last table *)
        (let initial_arith_row = [(NONE, SOME (0,255), s, res)] in
           SOME (process_guards_rec m_e 255 var_guards initial_arith_row))
-   | SOME (T, (SOME lv)) =>
+   | SOME (T, (SOME lv)) =>      (* here lv is unique *)
        case resolve_pd_max pd_type lv of
        | SOME max => 
            (let initial_arith_row = [(SOME lv, SOME (0,max), s, res)] in
               SOME (process_guards_rec m_e max var_guards initial_arith_row))
-       | _ => NONE  (* Impossible case by construction *)
+       | _ => NONE  (* this case needed in case it is unique but not defined *)
   )
 End
 
                         
-
-
 Definition convert_single_table_def:
   (convert_single_table [] m_e pd_type = SOME []) ∧
   (convert_single_table (line::tbl) m_e pd_type =
@@ -382,7 +258,6 @@ Definition convert_single_table_def:
             | NONE => NONE
             | SOME rest => SOME (res_line ++ rest)))
 End
-
 
 
 Definition convert_tables_def:
@@ -439,113 +314,39 @@ EVAL ``convert_tables ^policy1_var ^test_m_e ^test_pd_nested``;
 
 
 *)
-        
-
-(*
-val test_lval = ``lv_x "ttl"``;
-val test_atom = ``arithm_eq ^test_lval 5``;
-val test_m_e = ``[("x", ^test_atom)]``;
-val test_action = ``action "drop"``;
-val test_state = ``state 1``;
-
-(* PD type setups *)
-val test_pd_basic = ``[("ttl", type_length 4)]``;  (* 2^4-1 = 15 *)
-val test_pd_nested = ``[
-  ("hdr", type_record [
-    ("len", type_length 4);  (* 15 *)
-    ("flags", type_length 2) (* 3 *)
-  ])
-  ]``;
-
-
-val test_case1 = 
-  EVAL ``convert_single_table [([Var "x"], 1, ^test_action)] ^test_m_e ^test_pd_basic``;
-
-
-val test_case2 =
-  EVAL ``convert_single_table [([Not (Var "x")], 2, ^test_state)] ^test_m_e ^test_pd_basic``;
-
-val test_m_e_nested = ``[("y", arithm_eq (lv_acc (lv_x "hdr") "len") 5)]``;
-val test_case3 =
-  EVAL ``convert_single_table [([Var "y"], 3, ^test_action)] ^test_m_e_nested ^test_pd_nested``;
-
-val test_case4 =
-  EVAL ``convert_single_table [([Var "missing"], 4, ^test_state)] ^test_m_e ^test_pd_basic``;
-
-  
-val test_case5 =
-  EVAL ``convert_single_table [([Var "x"; Var "missing"], 5, ^test_action)] ^test_m_e ^test_pd_basic``;
-
-val test_case6 =
-  EVAL ``convert_single_table [([True; False], 6, ^test_state)] ^test_m_e ^test_pd_basic``;
-
-val test_case7 =
-  EVAL ``convert_single_table [([Var "x"; Not (Var "x")], 7, ^test_action)] ^test_m_e ^test_pd_basic``;
-
-val test_m_e_with_undefined = ``[("x", ^test_atom); ("missing", arithm_eq (lv_x "undefined") 0)]``;
-val test_case4a =
-  EVAL ``convert_single_table [([Var "missing"], 4, ^test_state)] ^test_m_e_with_undefined ^test_pd_basic``;
-
-
-(* Test data *)
-val test_tbl1 = ``[([Var "x"], (1:num), action "a")]``;
-val test_tbl2 = ``[([Not (Var "x")], (2:num), action "b")]``;
-val test_m_e = ``[("x", arithm_eq (lv_x "ttl") 5)]``;
-val test_pd = ``[("ttl", type_length 4)]``; (* MAX=15 *)
-
-(* Flattened version *)
-EVAL ``convert_tables [^test_tbl1; ^test_tbl2] ^test_m_e ^test_pd``;
-(* SOME [
-   [(SOME (lv_x "ttl"), SOME (5,5), 1, action "a")],
-   [(SOME (lv_x "ttl"), SOME (0,4), 2, state 1);
-    (SOME (lv_x "ttl"), SOME (6,15), 2, state 1)]
-] *)
-         
-*)
-
-
-
-
-
-                       
+    
+                  
 
 (* SEMANTICS *)
-
-
-
-
-
-
-
-Definition sem_interval_def:
-  (sem_interval (v:num) (SOME (lo, hi)) = (lo ≤ v ∧ v ≤ hi)) ∧
-  (sem_interval _ NONE = F)  (* False interval *)
-End
-
-
-(* Check if an interval row matches *)
 Definition is_intvl_match_row_def:
-  is_intvl_match_row (st_in:num) (st_num:num) (interval: (num # num) option) v =
-  
-    (st_in = st_num ∧ sem_interval v interval)
+  is_intvl_match_row  (s_in:num) (packet_input:pd) (row:('a intvl_row)) =
+    case row of
+      (SOME lval, SOME (a,b), s, res) =>
+        (case resolve_lval packet_input lval of
+           SOME (val_num v) =>  (a ≤ v ∧ v ≤ b ∧ (s_in = s))
+         | SOME _ => F  (* Non-numeric value *)
+         | NONE => F )   (* Lval not found *)
+    | (NONE, SOME (a,b), s, res) =>  (s_in = s)
+    | (NONE, NONE, s, res) =>  F
+    | (SOME lval, NONE, s, res) =>  F
 End
 
-
-
+        
 
 (* Process all rows in an interval table *)
 Definition check_all_intvl_rows_match_def:
-  check_all_intvl_rows_match st_in intvl_tbl v =
-  MAP (λ((lval_opt:arith_lv option ), intervall, st_num, res). 
-                  (is_intvl_match_row st_in st_num intervall v, (res:'a action_expr))) intvl_tbl
+  check_all_intvl_rows_match st_in intvl_tbl packet_input =
+  MAP (λ(lval_opt, intervall, st_num, res). 
+         (is_intvl_match_row st_in (packet_input:pd) (lval_opt , intervall, st_num, res)),
+          (res:'a action_expr)) intvl_tbl
 End
 
 
 
 (* Find first matching line in a converted table *)
 Definition match_intvl_tbl_def:
-  match_intvl_tbl (intvl_tbl: (('a intvl_row) list)) v st_in =
-  let lines_res = check_all_intvl_rows_match st_in intvl_tbl v in
+  match_intvl_tbl (intvl_tbl: (('a intvl_row) list)) packet_input st_in =
+  let lines_res = check_all_intvl_rows_match st_in intvl_tbl packet_input in
   case min_idx_till lines_res T of
     | SOME (idx, line) => SOME (SND line)
     | NONE => NONE
@@ -556,14 +357,14 @@ End
 
 (* Process list of interval tables with state propagation *)
 Definition match_intvl_tbll_def:
-  (match_intvl_tbll ([]: 'a intvl_table_list) _ _ = NONE) ∧
-  (match_intvl_tbll [intvl_tbl] v st_in =
-    case match_intvl_tbl intvl_tbl v st_in of
+  (match_intvl_tbll ([]: 'a intvl_table_list) packet_input st_in = NONE) ∧
+  (match_intvl_tbll [intvl_tbl] packet_input st_in =
+    case match_intvl_tbl intvl_tbl packet_input st_in of
       | SOME (action a) => SOME (action a)
       | _ => NONE) ∧
-  (match_intvl_tbll (intvl_tbl::intvl_tbls) v st_in =
-    case match_intvl_tbl intvl_tbl v st_in of
-      | SOME (state n) => match_intvl_tbll intvl_tbls v n
+  (match_intvl_tbll (intvl_tbl::intvl_tbls) packet_input st_in =
+    case match_intvl_tbl intvl_tbl packet_input st_in of
+      | SOME (state n) => match_intvl_tbll intvl_tbls packet_input n
       | _ => NONE)
 End
 
@@ -572,95 +373,111 @@ End
 
 (* Top-level interval table semantics *)
 Definition sem_intvl_tables_def:
-  sem_intvl_tables ((intvl_tbll: (('a intvl_table ) list)), st_in) v =
-  match_intvl_tbll intvl_tbll v st_in
+  sem_intvl_tables ((intvl_tbll: (('a intvl_table ) list)), st_in) (packet_input:pd) =
+  match_intvl_tbll intvl_tbll packet_input st_in
 End
 
 
+
+
+
+        
 (*
-val test_last_table = ``[
-  (SOME (lv_x "ttl"), SOME ((5:num),(10:num)), (1:num), action "accept");
-  (SOME (lv_x "ttl"), SOME (0,20), 1, action "reject")
-]``;
+val test_packet = “[("src_ip", val_num 192); ("dst_port", val_num 80)]”;
+val test_packet2 = “[("src_ip", val_num 10); ("dst_port", val_num 22)]”;
+val initial_state = “(0:num)”;
 
-EVAL ``sem_intvl_tables ([^test_last_table], 1) 7``; 
-EVAL ``sem_intvl_tables ([^test_last_table], 1) 15``;
+(* Test tables *)
+val test_table1 = ``[
+  (SOME (lv_x "dst_port"), SOME (75, 85), 0, state 1);
+  (NONE, SOME (0, 100), 0, state 2)
+] : (arith_lv option # (num # num) option # num # string action_expr) list``;
 
+  
+val test_table2 = ``[
+  (SOME (lv_x "src_ip"), SOME (190, 200), 1, action "allow_internal");
+  (NONE, NONE, 2, action "default_deny")
+] : (arith_lv option # (num # num) option # num # string action_expr) list``;
 
+(* Test table list with state transitions *)
+val test_tables = “[^test_table1; ^test_table2]: (arith_lv option # (num # num) option # num # string action_expr) list list”;
 
-
-
-val test_tables = ``[
-  (* Table 1: Accept small packets *)
-  [(SOME (lv_x "size"), SOME ((0:num),(500:num)), (1:num), state 2);
-   (SOME (lv_x "size"), SOME (501,1500), 1, state 2)];
-   
-  (* Table 2: Process medium packets *)  
-  [(SOME (lv_x "size"), SOME (501,1000), 3, state 4);
-   (SOME (lv_x "size"), SOME (900,1500), 2, state 5)];
-   
-  (* Table 3: Reject large packets *)
-  [(SOME (lv_x "size"), SOME (501,1000), 4, action "accept");
-   (SOME (lv_x "size"), SOME (501,1000), 5, action "reject")]
-]``;
+(* Test cases *)
+val test1 = EVAL ``sem_intvl_tables (^test_tables, ^initial_state) ^test_packet``;
+  *)               
 
 
-EVAL ``sem_intvl_tables (^test_tables, 1) 1000``;
+
+
+
+
+                   
+
+
+
+        
+
+
+(**********)
+(* proof *)
+(**********)
+
+
+
+
+
+Theorem convert_tables_never_empty:
+  ∀ h' t m_e packet_type.
+    convert_tables (h'::t) m_e packet_type ≠ SOME []
+Proof
+  rw[convert_tables_def] >>
+  rpt (BasicProvers.FULL_CASE_TAC >> gvs[]) 
+QED
+
+
+
+
+
+
+
+
+
+(*
+
+  ∀var_table m_e packet_input m_v interval_table packet_type st_in.
+ALL_DISTINCT (MAP FST m_e) ∧
+(∀var atom.  ALOOKUP m_e var = SOME atom ⇒
+             ALOOKUP m_v var = eval_arithm_atom packet_input atom) ∧
+convert_single_table var_table m_e packet_type = SOME interval_table ⇒
+match_tbl var_table m_v st_in = match_intvl_tbl interval_table packet_input st_in
+
+  
+  (* Process each line in the table *)
+  Induct_on `var_table` >> rw[] >>
+  rpt gen_tac >> strip_tac >>
+  fs[convert_single_table_def] >- (
+    (* Base case - empty table *)
+    fs[match_tbl_def, match_intvl_tbl_def, check_all_rows_match_def, 
+       check_all_intvl_rows_match_def]
+  ) >>
+  (* Inductive case *)
+  PairCases_on `h` >> fs[] >>
+  Cases_on `convert_line m_e packet_type (h0,h1,h2)` >> fs[] >>
+  rename1 `convert_line _ _ _ = SOME lines` >>
+  `∀line. MEM line lines ⇒ 
+         (is_match_row st_in h1 h0 m_v ⇔ 
+          is_intvl_match_row st_in packet_input line)` by (
+    (* Apply process_guard_semantics lemma *)
+    (* Need to show conditions hold for each guard in h0 *)
+  ) >>
+  (* Now relate the full table matching *)
+  fs[match_tbl_def, match_intvl_tbl_def] >>
+  (* Show check_all_rows_match and check_all_intvl_rows_match correspond *)
+  (* Prove min_idx_till returns equivalent results *)
 
 *)
 
 
-(*
-
-
-(* Evaluate left-value in packet structure *)
-Definition eval_lval_def:
-  (eval_lval pd (SOME lv) = resolve_lval pd lv) ∧
-  (eval_lval _ NONE = NONE)
-End
-
-(* Match a single interval row against packet *)
-Definition is_intvl_match_row_def:
-  is_intvl_match_row (st_in:num) (st_num:num) (lval_opt, interval: (num # num) option) pd =
-    case eval_lval pd lval_opt of
-      | SOME (val_num v) => (st_in = st_num ∧ sem_interval v interval)
-      | _ => F  (* Invalid lval or non-numeric value *)
-End
-
-(* Process all rows in table *)
-Definition check_all_intvl_rows_match_def:
-  check_all_intvl_rows_match st_in intvl_tbl pd =
-  MAP (λ(lval_opt, interval, st_num, res). 
-        (is_intvl_match_row st_in st_num (lval_opt, interval) pd, res)) intvl_tbl
-End
-
-(* Find first matching line *)
-Definition match_intvl_tbl_def:
-  match_intvl_tbl intvl_tbl pd st_in =
-  let lines_res = check_all_intvl_rows_match st_in intvl_tbl pd in
-  case min_idx_till lines_res T of
-    | SOME (idx, line) => SOME (SND line)
-    | NONE => NONE
-End
-
-(* Process table list with state propagation *)
-Definition match_intvl_tbll_def:
-  (match_intvl_tbll [] _ _ = NONE) ∧
-  (match_intvl_tbll [intvl_tbl] pd st_in =
-    case match_intvl_tbl intvl_tbl pd st_in of
-      | SOME (action a) => SOME (action a)
-      | _ => NONE) ∧
-  (match_intvl_tbll (intvl_tbl::intvl_tbls) pd st_in =
-    case match_intvl_tbl intvl_tbl pd st_in of
-      | SOME (state n) => match_intvl_tbll intvl_tbls pd n
-      | _ => NONE)
-End
-
-(* Top-level semantics *)
-Definition sem_intvl_tables_def:
-  sem_intvl_tables (intvl_tbll, st_in) pd =
-  match_intvl_tbll intvl_tbll pd st_in
-End
 
 
 
@@ -668,36 +485,53 @@ End
 
 
 
-
-
-
-
+                
         
-        
-
-(**********)
-(* proof *)
-
-
-
-
+               
 Theorem conversion_correctness:
-  ∀var_tables m_e packet_input m_v interval_tables.
+  ∀var_tables m_e packet_input m_v interval_tables packet_type st_in.
     ALL_DISTINCT (MAP FST m_e) ∧
     
     (∀var atom. 
        ALOOKUP m_e var = SOME atom ⇒ 
        ALOOKUP m_v var = eval_arithm_atom packet_input atom) ∧
     
-    (convert_tables var_tables m_e pd_type = SOME interval_tables) ⇒
+    (convert_tables var_tables m_e packet_type = SOME interval_tables) ⇒
     
     (* Semantic equivalence *)
     sem_tables (var_tables, st_in) m_v = 
     sem_intvl_tables (interval_tables, st_in) packet_input
 Proof
+  Induct >> rpt strip_tac >|[
+    (* empty table input*)
+    fs[convert_tables_def, sem_tables_def, sem_intvl_tables_def] >>
+    gvs[sem_tables_def, match_tbll_def, sem_intvl_tables_def, match_intvl_tbll_def] 
+    ,
+    fs[convert_tables_def] >>     
+    Cases_on ‘convert_single_table h m_e packet_type’ >> fs[] >>
+    Cases_on ‘convert_tables var_tables m_e packet_type’ >> fs[] >>
 
-cheat
+    last_x_assum (drule_all_then strip_assume_tac) >>
+    gvs[] >>
 
+    
+   ‘match_tbl h m_v st_in = match_intvl_tbl x packet_input st_in’ by (
+   cheat
+      ) >>
+
+    Cases_on ‘var_tables’ >>
+    Cases_on ‘x'’ >>
+    gvs[] >|[
+
+        (* both are last tables*)
+        fs[match_tbll_def, match_intvl_tbll_def]
+        ,
+        fs[convert_tables_def]
+        ,
+        gvs[convert_tables_never_empty]
+        ,
+        fs[match_tbll_def, match_intvl_tbll_def]
+      ]            
 QED
 
 
@@ -711,7 +545,7 @@ QED
 
 
 
-*)
+
 
 
 
